remove done

Hashtable.dfy
@@ -8,19 +8,11 @@ class Hashtable<K(==,!new),V(!new)> {
   ghost var mapa : map<K,Option<V>>;
 
   //1. All key-value pairs are in the appropriate bucket list
-  ghost predicate valid_hash_aux(len:int, l:List<(K,V)>, i:int)
-    requires 0 <= i < len
-  {
-    match l {
-      case Nil => true
-      case Cons((k,v),xs) => bucket(k, len) == i && valid_hash_aux(len, xs, i)
-    }
-  }
   ghost predicate valid_hash(d:array<List<(K,V)>>, i:int)
     requires 0 <= i < d.Length
     reads d
   {
-    valid_hash_aux(d.Length, d[i], i)
+    forall k, v :: mem((k,v), d[i]) ==> bucket(k, d.Length) == i
   }
   ghost predicate valid_pairs_bucket()
     reads this, data
@@ -34,7 +26,7 @@ class Hashtable<K(==,!new),V(!new)> {
     requires 0 < d.Length
   {
     var b := bucket(k, d.Length);
-    (k in m && m[k] == Some(v)) ==> mem((k,v), d[b]) && (k !in m) ==> !mem((k,v), d[b])
+    (k in m && m[k] == Some(v)) <==> mem((k,v), d[b])
   }
   ghost predicate valid_map()
     reads this, data
@@ -82,40 +74,10 @@ class Hashtable<K(==,!new),V(!new)> {
   }
 
   method rehash(arr: array<List<(K,V)>>, l : List<(K,V)>, index : int)
-    requires valid()
-    requires 0 <= index < arr.Length
-    modifies this, arr
-    ensures valid_hash(arr, index)
-  {
-    match l
-    case Nil => {}
-    case Cons((k, v), xs) => {
-      var b := bucket(k, arr.Length);
-      arr[b] := Cons((k,v), arr[b]);
-      mapa := mapa[k := Some(v)];
-      rehash(arr, xs, index);
-    }
-  }
+
 
   method resize()
-    requires valid()
-    modifies this, data
-    ensures valid()
-    ensures fresh(data)
-  {
-    var new_length := data.Length * 2;
-    var new_data := new List<(K,V)>[new_length](_ => Nil);
-    var i:int := 0;
-    while(i < data.Length)
-      invariant 0 <= i <= data.Length
-      invariant valid_hash(new_data, i)
-      modifies new_data
-    {
-      rehash(new_data, data[i], i);
-      i := i + 1;
-    }
-    data := new_data;
-  }
+    
 
   ghost function mem<T>(x:T, l:List<T>) : bool {
     match l {
@@ -164,41 +126,55 @@ class Hashtable<K(==,!new),V(!new)> {
       case Nil => Nil
       case Cons((k',v),xs) => if k==k' then list_remove(k,xs) else
       Cons((k',v),list_remove(k,xs))
-    } }
+    } 
+  }
 
   method remove(k: K)
-    modifies this, data
+    modifies this, data, `data
     requires valid()
     ensures valid()
-    ensures k !in mapa
-    ensures forall v :: !mem((k,v),data[bucket(k,data.Length)])
+    ensures k !in mapa || (k in mapa && mapa[k] == None)
   {
-    var kExists := find(k);
-    if(kExists != None) {
-      size := size - 1;
-    }
+
     var b := bucket(k, data.Length);
-    assert valid_hash_aux(data.Length, data[b], b);
-    data[b] := list_remove(k, data[b]);
-    mapa := mapa - {k};
-    assert valid_hash_aux(data.Length, old(data)[b], b);
-    assert bucket(k, data.Length) == b;
-    assert old(data).Length == data.Length;
+
+    match list_find(k, data[b]) {
+      case None => {
+        assert forall v :: !mem((k,v),data[bucket(k,data.Length)]);
+        assert forall k',v':: valid_data(k', v', mapa,data) && ((k' in mapa && mapa[k'] == Some(v')) <==> mem((k',v'), data[bucket(k', data.Length)]));
+        assert forall i:: 0 <= i < data.Length ==> valid_hash(data,i);
+        assert k !in mapa || (k in mapa && mapa[k] == None);
+      }
+      case Some(v) => {
+        assert forall k',v':: valid_data(k', v', mapa,data) && ((k' in mapa && mapa[k'] == Some(v')) <==> mem((k',v'),data[bucket(k', data.Length)]));       
+        data[b] := list_remove(k, data[b]);
+        mapa := mapa[k := None];
+        size := size - 1;
+       
+      }
+    }
   }
 
   method add(k: K,v: V)
-    modifies this, data
+    modifies this, data, `data
     requires valid()
     ensures valid()
-    ensures k in mapa ==> mapa[k] == Some(v)
-    ensures mem((k,v), data[bucket(k,data.Length)])
+    ensures k in mapa && mapa[k] == Some(v)
+    ensures size >= old(size)
   {
+    assert forall k', v' :: valid_data(k', v',mapa,data);
     var kExists := find(k);
     if(kExists == None) {
       size := size + 1;
     }
+    assert forall k',v':: valid_data(k', v', mapa,data) && ((k' in mapa && mapa[k'] == Some(v')) <==> mem((k',v'),data[bucket(k', data.Length)]));       
     var b := bucket(k, data.Length);
-    data[b] := Cons((k,v), data[b]);
+    data[b] := Cons((k,v), list_remove(k, data[b]));
     mapa := mapa[k := Some(v)];
+    assert mem((k,v), data[b]) && k in mapa;
+    assert bucket(k, data.Length) == b && mem((k,v), data[b]);
+    assert valid_data(k,v,mapa,data);
+
+
   }
 }
